---
title:  "Logarithm Theorems"
date: 2024-6-27 17:22:24 +0800
categories: logarithm
group: [logarithm]
---

## Theorem

$$
\begin{align}
\log_{b}MN &=\log_{b}M+\log_{b}N \\
\log_{b}\frac{M}{N} &=\log_{b}M-\log_{b}N \\
\log_{N}M &=\frac{log_{b}M}{\log_{b}N} \\
\log_{a}b\log_{b}c &=\log_{a}c \\
\log_{a^m}b^n &=\frac{n}{m}\log_{a}b \\
\log_{a}b &=\frac{1}{\log_{b}a} \\
\end{align}
$$

*note if $$a^b=c$$, then $$\log_{a}c=b$$*

## Proof
Rewrite exponetially
$$
\begin{align*}
b^x=M
b^y=N
b^(x+y)=MN  ???
\end{align*}
$$
